coq/CRun.v
@@ -1,0 +1,434 @@
+(* Concrete Algebra Procedure Execution as a Function
+
+Copyright (c) 2021 The MITRE Corporation
+
+This program is free software: you can redistribute it and/or
+modify it under the terms of the BSD License as published by the
+University of California. *)
+
+(** * Procedure Execution
+
+    This library contains a straightforward definition of the
+    semantics of procedure execution.  The semantics is specified
+    using a function.  The semantics of statement execution is defined
+    using a partial function that takes a runtime state and a list of
+    statements and returns the final runtime environment and a list of
+    terms that make up the procedure's outputs.  A runtime environment
+    is a map from program variables to terms.  A runtime state contains
+
+    - the current runtime environment,
+
+    - the current trace, and
+
+    - a list of the uniques that occur at the transmissions in the
+      current trace. *)
+
+Require Import FunInd Nat Bool Preamble Monad Proc Alg CSem.
+Import List.ListNotations.
+Open Scope list_scope.
+(** printing <- #←# *)
+
+(** A runtime state *)
+
+Record crun_state: Set :=
+  mkCRSt {
+      crenv: cenv;
+      crtr: list cevt;
+      cruniqs: list calg;
+      crs: list nat }.
+
+(** The semantics of expressions *)
+
+Definition crun_expr (rst: crun_state) (ex: expr):
+  option (crun_state * calg) :=
+  match ex with
+  | Quot_ s => Some (rst, CTg s)
+  | Hash_ v =>
+    x <- lookup v (crenv rst);;
+    Some (rst, CHs x)
+  | Pair_ u v =>
+    x <- lookup u (crenv rst);;
+    y <- lookup v (crenv rst);;
+    Some (rst, CPr x y)
+  | Encr_ u v =>
+    x <- lookup u (crenv rst);;
+    y <- lookup v (crenv rst);;
+    match crs rst with
+    | [] => Some (rst, CEn 0 x y)
+    | r :: rs =>
+      Some (mkCRSt (crenv rst)
+                   (crtr rst)
+                   (cruniqs rst)
+                   rs,
+            CEn r x y)
+    end
+  | Frst_ v =>
+    x <- lookup v (crenv rst);;
+    match x with
+    | CPr y z => Some (rst, y)
+    | _ => None
+    end
+  | Scnd_ v =>
+    x <- lookup v (crenv rst);;
+    match x with
+    | CPr y z => Some (rst, z)
+    | _ => None
+    end
+  | Decr_ u v =>
+    x <- lookup u (crenv rst);;
+    match x with
+    | CEn _ y z =>
+      k <- lookup v (crenv rst);;
+      if negb (chas_enc k) && calg_eqb k (cinv z) then
+        Some (rst, y)
+      else
+        None
+    | _ => None
+    end
+  | Recv_ v =>
+    c <- lookup v (crenv rst);;
+    match crtr rst with
+    | CRv d x :: tr =>
+      match c with
+      | CCh n =>
+        if n =? d then
+          Some (mkCRSt (crenv rst) tr (cruniqs rst) (crs rst), x)
+        else
+          None
+      | _ => None
+      end
+    | _ => None
+    end
+  | Frsh =>
+    match cruniqs rst with
+    | u :: us =>
+      Some (mkCRSt (crenv rst) (crtr rst) us (crs rst), u)
+    | _ => None
+    end
+  end.
+
+Lemma crun_expr_env_extends:
+  forall rst ex rst' val,
+    crun_expr rst ex = Some (rst', val) ->
+    crenv rst' = crenv rst.
+Proof.
+  intros.
+  destruct ex; simpl in H; inv H; auto.
+  - apply do_some in H1.
+    destruct H1.
+    destruct H.
+    inv H0; auto.
+  - apply do_some in H1.
+    destruct H1.
+    destruct H.
+    apply do_some in H0.
+    destruct H0.
+    destruct H0.
+    inv H1; auto.
+  - destruct (lookup n (crenv rst)).
+    + destruct (lookup n0 (crenv rst)).
+      * destruct (crs rst); inv H1; auto.
+      * inv H1.
+    + inv H1.
+  - destruct (lookup n (crenv rst)).
+    + destruct c; inv H1; auto.
+    + inv H1.
+  - destruct (lookup n (crenv rst)).
+    + destruct c; inv H1; auto.
+    + inv H1.
+  - destruct (lookup n (crenv rst)).
+    + destruct c; inv H1; auto.
+      destruct (lookup n0 (crenv rst)); inv H0; auto.
+      destruct (negb (chas_enc c) && calg_eqb c (cinv c2)); inv H1; auto.
+    + inv H1.
+  - destruct (cruniqs rst); inv H1; auto.
+  - destruct (lookup n (crenv rst)); inv H1; auto.
+    destruct (crtr rst); inv H0; auto.
+    destruct c0; inv H1; auto.
+    destruct c; inv H0; auto.
+    destruct (n1 =? n0); inv H1; auto.
+Qed.
+
+(** Check that the type of [x] is compatible with [t]. *)
+
+Definition ctype_check (x: calg) (t: type): bool :=
+  type_eqb t Mesg || type_eqb (ctype_of x) t.
+
+(** The semantics of statements *)
+
+Definition crun_stmt (rst: crun_state) (cmd: stmt): option crun_state :=
+  match cmd with
+  | Bind (v, t) exp =>
+    sx <- crun_expr rst exp;;
+    let (rst, x) := sx in
+    if ctype_check x t then
+      Some (mkCRSt
+              ((v, x) :: crenv rst)
+              (crtr rst)
+              (cruniqs rst)
+              (crs rst))
+    else
+      None
+   | Send u v =>
+     match crtr rst with
+     | CSd d x :: tr =>
+       c <- lookup u (crenv rst);;
+       match c with
+       | CCh n =>
+         if n =? d then
+           y <- lookup v (crenv rst);;
+           if calg_eqb x y then
+             Some (mkCRSt (crenv rst) tr (cruniqs rst) (crs rst))
+           else
+             None
+         else
+           None
+       | _ => None
+       end
+     | _ => None
+    end
+  | Same u v =>
+    x <- lookup u (crenv rst);;
+    y <- lookup v (crenv rst);;
+    if negb (chas_enc x) && calg_eqb x y then
+      Some rst
+    else
+      None
+  | Ltkp u v w =>
+    x <- lookup u (crenv rst);;
+    y <- lookup v (crenv rst);;
+    z <- lookup w (crenv rst);;
+    match y, z with
+    | CNm b, CNm c =>
+      if calg_eqb x (CSk (Lt b c)) then
+        Some rst
+      else
+        None
+    | _, _ => None
+    end
+  | Invp u v =>
+    x <- lookup u (crenv rst);;
+    y <- lookup v (crenv rst);;
+    if negb (chas_enc x) && calg_eqb x (cinv y) then
+      Some rst
+    else
+      None
+  | Namp u v =>
+    x <- lookup u (crenv rst);;
+    y <- lookup v (crenv rst);;
+    match x, y with
+    | CAk k, CNm b =>
+      if akey_eqb k (Pb b) then
+        Some rst
+      else
+        None
+    | CIk k, CNm b =>
+      if akey_eqb k (Pb b) then
+        Some rst
+      else
+        None
+    | _, _ => None
+    end
+  | Nm2p u v w =>
+    x <- lookup u (crenv rst);;
+    y <- lookup v (crenv rst);;
+    z <- lookup w (crenv rst);;
+    match x, y, z with
+    | CAk k, CTg s, CNm c =>
+      if akey_eqb k (Pb2 s c) then
+        Some rst
+      else
+        None
+    | CIk k, CTg s, CNm c =>
+      if akey_eqb k (Pb2 s c) then
+        Some rst
+      else
+        None
+    | _, _, _ => None
+    end
+  | Return _ => None
+end.
+
+Lemma crun_stmt_env_extends:
+  forall rst stmt rst',
+    crun_stmt rst stmt = Some rst' ->
+    exists ev, crenv rst' = ev ++ crenv rst.
+Proof.
+  intros.
+  destruct stmt; simpl in H.
+  - inv H.
+  - destruct d.
+    alt_option_dec (crun_expr rst e) p G; rewrite G in H.
+    + inv H.
+    + expand_let_pairs.
+      destruct p.
+      apply crun_expr_env_extends in G.
+      simpl in H.
+      destruct (ctype_check c0 t); inv H; auto.
+      exists [(n, c0)]; simpl.
+      rewrite G.
+      auto.
+  - exists []; simpl.
+    destruct (crtr rst).
+    inv H.
+    destruct c.
+    + destruct (lookup n (crenv rst)).
+      * destruct c0; try inv H.
+        destruct (n2 =? n1).
+        -- destruct (lookup n0 (crenv rst)).
+           ++ destruct (calg_eqb c c0); inv H1; simpl; auto.
+           ++ inv H1.
+        -- inv H1.
+      * inv H.
+    + inv H.
+  - exists []; simpl.
+    destruct (lookup n (crenv rst)).
+    + destruct (lookup n0 (crenv rst)).
+      * destruct (negb (chas_enc c) && calg_eqb c c0); inv H; simpl; auto.
+      * inv H.
+    + inv H.
+  - exists []; simpl.
+    destruct (lookup n (crenv rst)); inv H; auto.
+    destruct (lookup n0 (crenv rst)); inv H1; auto.
+    destruct (lookup n1 (crenv rst)); inv H0; auto.
+    destruct c0; inv H1; auto.
+    destruct c1; inv H0; auto.
+    destruct (calg_eqb c (CSk (Lt n2 n3))); inv H1; auto.
+  - exists []; simpl.
+    destruct (lookup n (crenv rst)); inv H; auto.
+    destruct (lookup n0 (crenv rst)); inv H1; auto.
+    destruct (negb (chas_enc c) && calg_eqb c (cinv c0)); inv H0; auto.
+  - exists []; simpl.
+    destruct (lookup n (crenv rst)); inv H; auto.
+    destruct (lookup n0 (crenv rst)); inv H1; auto.
+    destruct c; inv H0; auto.
+    + destruct c0; inv H1; auto.
+      destruct (akey_eqb a (Pb n1)); inv H0; auto.
+    + destruct c0; inv H1; auto.
+      destruct (akey_eqb a (Pb n1)); inv H0; auto.
+  - exists []; simpl.
+    destruct (lookup n (crenv rst)); inv H; auto.
+    destruct (lookup n0 (crenv rst)); inv H1; auto.
+    destruct (lookup n1 (crenv rst)); inv H0; auto.
+    destruct c; inv H1; auto.
+    + destruct c0; inv H0; auto.
+      destruct c1; inv H1; auto.
+      destruct (akey_eqb a (Pb2 s n2)); inv H0; auto.
+    + destruct c0; inv H0; auto.
+      destruct c1; inv H1; auto.
+      destruct (akey_eqb a (Pb2 s n2)); inv H0; auto.
+Qed.
+
+(** The semantics of lists of statements *)
+
+Fixpoint crun_stmts (rst: crun_state) (stmts: list stmt):
+  option (cenv * list calg) :=
+  match stmts with
+  | [] => None
+  | [Return vs] =>
+    match crtr rst, cruniqs rst with
+    | [], [] =>
+      xs <- map_m (fun x => lookup x (crenv rst)) vs;;
+      Some (crenv rst, xs)
+    | _, _ => None
+    end
+  | cmd :: stmts =>
+    rst <- crun_stmt rst cmd;;
+    crun_stmts rst stmts
+  end.
+
+Lemma crun_stmts_env_extends:
+  forall rst stmts ev outs,
+    crun_stmts rst stmts = Some (ev, outs) ->
+    exists ev', ev = ev' ++ crenv rst.
+Proof.
+  intros rst stmts.
+  revert rst.
+  induction stmts; intros.
+  - simpl in H.
+    inv H.
+  - destruct a; unfold crun_stmts in H; fold crun_stmts in H.
+    + exists []; simpl.
+      destruct stmts; inv H; auto.
+      destruct (crtr rst); inv H1; auto.
+      destruct (cruniqs rst); inv H0; auto.
+      destruct (map_m (fun x : nat => lookup x (crenv rst)) l); inv H1; auto.
+    + apply do_some in H.
+      repeat destruct_ex_and.
+      apply crun_stmt_env_extends in H.
+      apply IHstmts in H0.
+      repeat destruct_ex_and; subst.
+      rewrite H.
+      exists (x0 ++ x1).
+      rewrite app_assoc; auto.
+    + apply do_some in H.
+      repeat destruct_ex_and.
+      apply crun_stmt_env_extends in H.
+      apply IHstmts in H0.
+      repeat destruct_ex_and; subst.
+      rewrite H.
+      exists (x0 ++ x1).
+      rewrite app_assoc; auto.
+    + apply do_some in H.
+      repeat destruct_ex_and.
+      apply crun_stmt_env_extends in H.
+      apply IHstmts in H0.
+      repeat destruct_ex_and; subst.
+      rewrite H.
+      exists (x0 ++ x1).
+      rewrite app_assoc; auto.
+    + apply do_some in H.
+      repeat destruct_ex_and.
+      apply crun_stmt_env_extends in H.
+      apply IHstmts in H0.
+      repeat destruct_ex_and; subst.
+      rewrite H.
+      exists (x0 ++ x1).
+      rewrite app_assoc; auto.
+    + apply do_some in H.
+      repeat destruct_ex_and.
+      apply crun_stmt_env_extends in H.
+      apply IHstmts in H0.
+      repeat destruct_ex_and; subst.
+      rewrite H.
+      exists (x0 ++ x1).
+      rewrite app_assoc; auto.
+    + apply do_some in H.
+      repeat destruct_ex_and.
+      apply crun_stmt_env_extends in H.
+      apply IHstmts in H0.
+      repeat destruct_ex_and; subst.
+      rewrite H.
+      exists (x0 ++ x1).
+      rewrite app_assoc; auto.
+    + apply do_some in H.
+      repeat destruct_ex_and.
+      apply crun_stmt_env_extends in H.
+      apply IHstmts in H0.
+      repeat destruct_ex_and; subst.
+      rewrite H.
+      exists (x0 ++ x1).
+      rewrite app_assoc; auto.
+Qed.
+
+(** Bind inputs with procedure parameters. *)
+
+Fixpoint cbind_inputs (ds: list decl) (xs: list calg) (renv: cenv):
+  option cenv :=
+  match ds, xs with
+  | [], [] => Some renv
+  | (v, t) :: ds, x :: xs =>
+    if ctype_check x t then
+      cbind_inputs ds xs ((v, x) :: renv)
+    else
+      None
+  | _, _ => None
+  end.
+
+(** The semantics of a procedure *)
+
+Definition crun (p: proc) (inputs: list calg) (tr: list cevt)
+           (us: list calg) (rs: list nat):
+  option (cenv * list calg) :=
+  renv <- cbind_inputs (ins p) inputs [];;
+  crun_stmts (mkCRSt (rev renv) tr us rs) (body p).
